Simplify olty: don't require values to be closed

theories/olty.v
@@ -20,21 +20,8 @@ Section olty_limit_preserving.
     apply bi.limit_preserving_Persistent => n f g Heq. exact: Heq.
   Qed.
 
-  Definition vclosed (A : hoEnvD Σ i) := ∀ args ρ v, A args ρ v ⊢ ⌜ nclosed_vl v 0 ⌝.
-
-  Instance: LimitPreserving vclosed.
-  Proof.
-    apply limit_preserving_forall=> args;
-    apply limit_preserving_forall=> ρ; apply limit_preserving_forall=> w.
-    apply limit_preserving_entails; last apply _.
-    move => n f g Heq. exact: Heq.
-  Qed.
-
-  Definition restrict A := vclosed A ∧ hoEnvD_persistent A.
-  Global Instance: LimitPreserving restrict.
-  Proof.
-    apply limit_preserving_and; apply _.
-  Qed.
+  Definition restrict A := hoEnvD_persistent A.
+  Global Instance: LimitPreserving restrict := _.
 End olty_limit_preserving.
 
 (**
@@ -43,12 +30,10 @@ and values. Adapted from
 https://gitlab.mpi-sws.org/iris/examples/blob/d4f4153920ea82617c7222aeeb00b6710d51ee03/theories/logrel_heaplang/ltyping.v#L5. *)
 Record olty Σ i := Olty {
   olty_car :> vec vl i → (var → vl) → vl → iProp Σ;
-  olty_vclosed : vclosed olty_car;
   olty_persistent args ρ v : Persistent (olty_car args ρ v);
 }.
-Global Arguments Olty {_ _} _%I _ {_}.
+Global Arguments Olty {_ _} _%I {_}.
 Global Arguments olty_car {_ _} _ _ _ _: simpl never.
-Global Arguments olty_vclosed {_ _} _ _ _.
 Bind Scope olty_scope with olty.
 Delimit Scope olty_scope with T.
 Global Existing Instance olty_persistent.
@@ -74,38 +59,34 @@ Section olty_ofe.
   (* Only needed to define Olty using Iris fixpoints (e.g. for normal recursive types). *)
   Global Instance olty_cofe : Cofe oltyO.
   Proof.
-    set curry_olty : ∀ A, restrict A → olty Σ i := λ A '(conj P1 P2), @Olty Σ i A P1 P2.
-    apply (iso_cofe_subtype' restrict curry_olty olty_car) => //.
+    apply (iso_cofe_subtype' restrict Olty olty_car) => //.
     - by move => [].
-    - by move => ? [].
     - apply _.
   Qed.
 
-  Global Program Instance olty_inhabited : Inhabited (olty Σ i) := populate (Olty (λ _ _ _, False)%I _).
-  Next Obligation. by unseal=>?. Qed.
+  Global Program Instance olty_inhabited : Inhabited (olty Σ i) := populate (Olty (λ _ _ _, False)%I).
 
   Global Instance olty_car_ne : NonExpansive oApp.
   Proof. intros n f g Heq. apply Heq. Qed.
   Global Instance lty_car_proper : Proper ((≡) ==> (≡)) oApp.
   Proof. apply ne_proper, olty_car_ne. Qed.
 
-  Program Definition pack φ (Hvc : vclosed φ) := Olty (λ args ρ v, □ φ args ρ v)%I _.
-  Next Obligation. rewrite /vclosed; intros. iIntros "?". by iApply Hvc. Qed.
+  Program Definition pack φ := Olty (λ args ρ v, □ φ args ρ v)%I.
 
   Lemma persistently_id (P : iProp Σ) `{!Persistent P}: □P ⊣⊢ P.
   (* Proof. by iSplit; iIntros. Qed. *)
   Proof. apply: intuitionistic_intuitionistically. Qed.
 
-  Lemma olty_car_pack_id φ (H : vclosed φ) `{∀ args ρ v, Persistent (φ args ρ v)} :
-    oApp (pack φ H) ≡ φ.
+  Lemma olty_car_pack_id φ `{∀ args ρ v, Persistent (φ args ρ v)} :
+    oApp (pack φ) ≡ φ.
   Proof.
     move => ??? /=.
     apply: intuitionistic_intuitionistically.
   Qed.
 
-  Lemma pack_olty_car_id τ : pack (olty_car τ) (olty_vclosed τ) ≡ τ.
+  Lemma pack_olty_car_id τ : pack (olty_car τ) ≡ τ.
   Proof.
-    move: τ => [τ Hp Hvc] args ρ v; rewrite /olty_car/=.
+    move: τ => [τ Hp] args ρ v; rewrite /olty_car/=.
     apply: intuitionistic_intuitionistically.
   Qed.
 
@@ -129,24 +110,38 @@ Section olty_ofe.
 
   Lemma olty_eq τ1 τ2: olty_car τ1 = olty_car τ2 → τ1 = τ2.
   Proof.
-    move: τ1 τ2 => [φ1 Hp1 Hvc1] [φ2 Hp2 Hvc2]. rewrite /olty_car /=.
+    move: τ1 τ2 => [φ1 Hp1] [φ2 Hp2]. rewrite /olty_car /=.
     intros ->. f_equal; exact: ProofIrrelevance.proof_irrelevance.
   Qed.
 
   Global Instance ids_olty : Ids (olty Σ i) := λ _, inhabitant.
   Global Program Instance rename_olty : Rename (olty Σ i) :=
-    λ r τ, Olty (rename r (olty_car τ)) _.
-  Next Obligation. rewrite /vclosed; intros. exact: olty_vclosed. Qed.
+    λ r τ, Olty (rename r (olty_car τ)).
   Global Program Instance hsubst_olty : HSubst vl (olty Σ i) :=
-    λ sb τ, Olty ((olty_car τ).|[sb]) (_ (olty_car τ).|[sb]).
-  Next Obligation. rewrite /vclosed; intros. exact: olty_vclosed. Qed.
+    λ sb τ, Olty (olty_car τ).|[sb].
 
   Global Instance hsubstLemmas_olty : HSubstLemmas vl (olty Σ i).
   Proof.
-    split=> [s|??|?? s]; apply olty_eq => //; case: s => [φ??];
+    split=> [s|??|?? s]; apply olty_eq => //; case: s => [φ?];
     rewrite /hsubst /hsubst_olty /olty_car.
     all: trivial using hsubst_id, id_hsubst, hsubst_comp.
   Qed.
+
+  Lemma olty_subst_compose_ind τ args ρ1 ρ2 v: τ.|[ρ1] args ρ2 v ⊣⊢ τ args (ρ1 >> ρ2) v.
+  Proof. done. Qed.
+
+  Lemma olty_subst_compose τ args ρ1 ρ2 ρ3 :
+    ρ1 >> ρ2 = ρ3 → oApp τ.|[ρ1] args ρ2 ≡ oApp τ args ρ3.
+  Proof. by move=> <-. Qed.
+
+  Lemma olty_weaken_one τ args ρ:
+     oApp τ.|[ren (+1)] args ρ ≡ oApp τ args (stail ρ).
+  Proof. apply olty_subst_compose. autosubst. Qed.
+
+  Lemma olty_subst_one τ v w args ρ:
+    oApp τ.|[v/] args ρ w ≡ oApp τ args (v.[ρ] .: ρ) w.
+  Proof. apply olty_subst_compose. autosubst. Qed.
+
 
 (* Global Instance rename_olty2 : Rename (olty Σ i) :=
     λ r τ, Olty (λ ρ, τ (r >>> ρ)) (λ ρ, olty_vclosed τ _).
@@ -159,28 +154,6 @@ Section olty_ofe.
     rewrite /hsubst /hsubst_olty2 /olty_car /=.
     all: by asimpl.
   Qed. *)
-
-  Lemma hoEnvD_weaken ρ1 ρ2 ρ3 φ args :
-    φ.|[upn (length ρ1) (ren (+ length ρ2))] args (to_subst (ρ1 ++ ρ2 ++ ρ3))
-    = φ args (to_subst (ρ1 ++ ρ3)).
-  Proof. rewrite /hsubst_hoEnvD /hsubst to_subst_weaken //. Qed.
-
-  Lemma olty_weaken ρ1 ρ2 ρ3 τ args :
-    τ.|[upn (length ρ1) (ren (+ length ρ2))] args (to_subst (ρ1 ++ ρ2 ++ ρ3))
-    = τ args (to_subst (ρ1 ++ ρ3)).
-  Proof.
-    (* rewrite /hsubst_olty /hsubst_hoEnvD /hsubst /= to_subst_weaken //. *)
-    rewrite [@hsubst _ _ hsubst_olty]/hsubst /hsubst_olty /=.
-    exact: hoEnvD_weaken.
-  Qed.
-
-  Lemma hoEnvD_weaken_one v φ ρ args :
-    φ.|[ren (+1)] args (v .: to_subst ρ) = φ args (to_subst ρ).
-  Proof. by rewrite (hoEnvD_weaken [] [v]). Qed.
-
-  Lemma olty_weaken_one v τ ρ args :
-    oApp τ.|[ren (+1)] args (v .: to_subst ρ) ≡ τ args (to_subst ρ).
-  Proof. by rewrite (olty_weaken [] [v]). Qed.
 End olty_ofe.
 
 Notation oClose φ := (olty_car φ vnil : envD _).
@@ -195,116 +168,54 @@ Section olty_ofe_2.
     | φ :: Γ' => env_oltyped Γ' (stail ρ) ∧ oClose φ ρ (ρ 0)
     | nil => True
     end%I.
+  Notation "⟦ Γ ⟧*" := (env_oltyped Γ).
 
   Global Instance env_oltyped_persistent (Γ : sCtx) ρ: Persistent (env_oltyped Γ ρ).
   Proof. elim: Γ ρ => [|τ Γ IHΓ] ρ /=; apply _. Qed.
 
-  Lemma env_oltyped_cl_ρ Γ ρ :
-    env_oltyped Γ ρ -∗ ⌜ nclosed_sub (length Γ) 0 ρ ⌝.
-  Proof.
-    elim: Γ ρ => [|φ Γ IHΓ] ρ /=; [| rewrite IHΓ olty_vclosed ]; iIntros "!% //".
-    - move => [Hclρ Hclp0] [|n /lt_S_n] Hle. exact Hclp0. apply Hclρ, Hle.
-  Qed.
-
-  Lemma env_oltyped_cl_app `{Sort X} (x : X) Γ ρ:
-    env_oltyped Γ ρ -∗
-    ⌜ nclosed x (length Γ) ⌝ → ⌜ nclosed x.|[ρ] 0 ⌝.
-  Proof. rewrite env_oltyped_cl_ρ. iIntros "!%". exact: nclosed_sub_app. Qed.
-
-  Lemma env_oltyped_cl_app_vl v Γ ρ:
-    env_oltyped Γ ρ -∗
-    ⌜ nclosed_vl v (length Γ) ⌝ → ⌜ nclosed_vl v.[ρ] 0 ⌝.
-  Proof. rewrite env_oltyped_cl_ρ. iIntros "!%". exact: nclosed_sub_app_vl. Qed.
-
-  Fixpoint env_oltyped_fin (Γ : sCtx) vs : iProp Σ :=
-    match Γ, vs with
-    | φ :: Γ', v :: vs => env_oltyped_fin Γ' vs ∧ oClose φ (v .: to_subst vs) v
-    | nil, nil => True
-    | _, _ => False
-    end%I.
-  Notation "⟦ Γ ⟧*" := (env_oltyped_fin Γ).
-
-  Global Instance env_oltyped_fin_persistent (Γ : sCtx) vs: Persistent (⟦ Γ ⟧* vs).
-  Proof. elim: Γ vs => [|τ Γ IHΓ] [|v vs] /=; apply _. Qed.
-
-  Lemma env_oltyped_transl Γ vs :
-    ⟦ Γ ⟧* vs -∗ env_oltyped Γ (to_subst vs).
-  Proof.
-    elim: Γ vs => [|Γ φ IHΓ] [|v vs] /=;
-      by [ | iIntros "[]"| asimpl; rewrite IHΓ ].
-  Qed.
-
-  Lemma env_oltyped_fin_cl_ρ Γ ρ:
-    ⟦ Γ ⟧* ρ -∗ ⌜ nclosed_sub (length Γ) 0 (to_subst ρ) ⌝.
-  Proof. rewrite env_oltyped_transl env_oltyped_cl_ρ //. Qed.
-
-  Lemma env_oltyped_fin_cl_app `{Sort X} (x : X) Γ ρ:
-    ⟦ Γ ⟧* ρ -∗
-    ⌜ nclosed x (length Γ) ⌝ → ⌜ nclosed x.|[to_subst ρ] 0 ⌝.
-  Proof. rewrite env_oltyped_transl (env_oltyped_cl_app x) //. Qed.
-
-  Lemma env_oltyped_fin_cl_app_vl v Γ ρ:
-    ⟦ Γ ⟧* ρ -∗
-    ⌜ nclosed_vl v (length Γ) ⌝ → ⌜ nclosed_vl v.[to_subst ρ] 0 ⌝.
-  Proof. rewrite env_oltyped_transl env_oltyped_cl_app_vl //. Qed.
-
-  Lemma interp_env_ρ_closed Γ ρ: ⟦ Γ ⟧* ρ -∗ ⌜ cl_ρ ρ ⌝.
-  Proof.
-    elim: Γ ρ => [|τ Γ IHΓ] [|v ρ] //=; try by iIntros "!%".
-    rewrite IHΓ olty_vclosed. iIntros "!%". intuition.
-  Qed.
-
   Lemma interp_env_lookup Γ ρ (τ : olty Σ 0) x:
     Γ !! x = Some τ →
-    ⟦ Γ ⟧* ρ -∗ oClose τ.|[ren (+x)] (to_subst ρ) (to_subst ρ x).
+    ⟦ Γ ⟧* ρ -∗ oClose τ.|[ren (+x)] ρ (ρ x).
   Proof.
-    elim: Γ ρ x => [//|τ' Γ' IHΓ] [|v ρ] x Hx /=. by iIntros "[]".
+    elim: Γ ρ x => [//|τ' Γ' IHΓ] ρ x Hx /=.
     iDestruct 1 as "[Hg Hv]". move: x Hx => [ [->] | x Hx] /=.
     - rewrite hsubst_id. by [].
     - rewrite hrenS.
-      iApply (olty_weaken_one v (τ.|[ren (+x)]) ρ).
-      iApply (IHΓ ρ x Hx with "Hg").
+      iApply (olty_weaken_one (τ.|[ren (+x)])).
+      iApply (IHΓ (stail ρ) x Hx with "Hg").
   Qed.
 
-  Program Definition ho_closed_olty {i} (φ : hoEnvD Σ i) `{∀ args ρ v, Persistent (φ args ρ v)} : olty Σ i :=
-    Olty (λ args ρ v, ⌜ nclosed_vl v 0 ⌝ ∧ φ args ρ v)%I _.
-  Next Obligation. iIntros (??????) "[$_]". Qed.
-
-  Definition closed_olty (φ : envD Σ)`{∀ ρ v, Persistent (φ ρ v)} : olty Σ 0 :=
-    ho_closed_olty (vopen φ).
+  Definition olty0 (φ : envD Σ)`{∀ ρ v, Persistent (φ ρ v)} : olty Σ 0 :=
+    Olty (vopen φ).
 
   (** We can define once and for all basic "logical" types: top, bottom, and, or, later and μ. *)
-  Definition oTop : olty Σ i := ho_closed_olty (λ args ρ v, True)%I.
+  Definition oTop : olty Σ i := Olty (λ args ρ v, True)%I.
 
-  Program Definition oBot : olty Σ i := Olty (λ args ρ v, False)%I _.
-  Next Obligation. intros **?**. exact: False_elim. Qed.
+  Program Definition oBot : olty Σ i := Olty (λ args ρ v, False)%I.
 
-  Program Definition oAnd τ1 τ2 : olty Σ i := Olty (λ args ρ v, τ1 args ρ v ∧ τ2 args ρ v)%I _.
-  Next Obligation. intros **?**. rewrite olty_vclosed. iIntros "[$ _]". Qed.
+  Program Definition oAnd τ1 τ2 : olty Σ i := Olty (λ args ρ v, τ1 args ρ v ∧ τ2 args ρ v)%I.
 
-  Program Definition oOr τ1 τ2 : olty Σ i := Olty (λ args ρ v, τ1 args ρ v ∨ τ2 args ρ v)%I _.
-  Next Obligation. intros **?**. rewrite !olty_vclosed. iIntros "[$ | $]". Qed.
+  Program Definition oOr τ1 τ2 : olty Σ i := Olty (λ args ρ v, τ1 args ρ v ∨ τ2 args ρ v)%I.
 
   Definition eLater n (φ : hoEnvD Σ i) : hoEnvD Σ i := (λ args ρ v, ▷^n φ args ρ v)%I.
-  Definition oLater τ := ho_closed_olty (eLater 1 τ).
+  Definition oLater τ := Olty (eLater 1 τ).
 
-  Program Definition ho_oMu {i} (τ : olty Σ i) : olty Σ i := Olty (λ args ρ v, τ args (v .: ρ) v) _.
-  Next Obligation. rewrite /vclosed; intros. exact: olty_vclosed. Qed.
+  Program Definition ho_oMu {i} (τ : olty Σ i) : olty Σ i := Olty (λ args ρ v, τ args (v .: ρ) v).
 
   Definition oMu (τ : olty Σ 0) : olty Σ 0 := ho_oMu τ.
 
-  Lemma interp_TMu_ren (T : olty Σ i) args ρ v: ho_oMu T.|[ren (+1)] args (to_subst ρ) v ≡ T args (to_subst ρ) v.
-  Proof. rewrite [_ (ho_oMu _)]/olty_car /= (olty_weaken_one v T ρ args v). by []. Qed.
+  Lemma interp_TMu_ren (T : olty Σ i) args ρ v: ho_oMu T.|[ren (+1)] args ρ v ≡ T args ρ v.
+  Proof. rewrite [_ (ho_oMu _)]/olty_car /= (olty_weaken_one T args _ v). by []. Qed.
 
   Definition interp_expr `{dlangG Σ} (φ : hoEnvD Σ 0) : envPred tm Σ :=
     λ ρ t, WP t {{ vclose φ ρ }} %I.
   Global Arguments interp_expr /.
 
   Definition oTSel0 `{dlangG Σ} s σ :=
-    closed_olty (λ ρ v, ∃ ψ, s ↗[ σ ] ψ ∧ ▷ □ ψ v)%I.
+    olty0 (λ ρ v, ∃ ψ, s ↗[ σ ] ψ ∧ ▷ □ ψ v)%I.
 End olty_ofe_2.
 
-Notation "⟦ Γ ⟧*" := (env_oltyped_fin Γ).
+Notation "⟦ Γ ⟧*" := (env_oltyped Γ).
 Arguments oltyO : clear implicits.
 End OLty.
 
@@ -315,17 +226,16 @@ Section judgments.
   Implicit Types (τ : olty Σ 0).
 
   Definition step_indexed_ivstp Γ τ1 τ2 i j: iProp Σ :=
-    (□∀ ρ v, ⌜ nclosed_vl v 0 ⌝ →
-      ⟦Γ⟧*ρ → (▷^i oClose τ1 (to_subst ρ) v) → ▷^j oClose τ2 (to_subst ρ) v)%I.
+    □∀ ρ v,
+      ⟦Γ⟧*ρ → ▷^i oClose τ1 ρ v → ▷^j oClose τ2 ρ v.
   Global Arguments step_indexed_ivstp /.
 
-  Definition ietp Γ τ e : iProp Σ := (⌜ nclosed e (length Γ) ⌝ ∧
-    □∀ ρ, ⟦Γ⟧* ρ → interp_expr τ (to_subst ρ) (e.|[to_subst ρ]))%I.
+  Definition ietp Γ τ e : iProp Σ :=
+    □∀ ρ, ⟦Γ⟧* ρ → interp_expr τ ρ (e.|[ρ]).
   Global Arguments ietp /.
 
   Definition step_indexed_ietp Γ τ e i: iProp Σ :=
-    (⌜ nclosed e (length Γ) ⌝ ∧ □∀ ρ, ⟦Γ⟧* ρ →
-      interp_expr (eLater i τ) (to_subst ρ) (e.|[to_subst ρ]))%I.
+    □∀ ρ, ⟦Γ⟧* ρ → interp_expr (eLater i τ) ρ (e.|[ρ]).
   Global Arguments step_indexed_ietp /.
 
 End judgments.
@@ -339,27 +249,24 @@ Section typing.
   Implicit Types (τ : olty Σ 0).
 
   Lemma iterate_TLater_later i τ ρ v:
-    nclosed_vl v 0 →
     oClose (iterate oLater i τ) ρ v ≡ (vclose (eLater i τ) ρ v).
   Proof.
-    elim: i => [|i IHi] // => Hcl. rewrite iterate_S [_ ρ]/olty_car/= /eLater IHi //.
-    iSplit; by [iIntros "#[_ $]" | iIntros "$"].
+    elim: i => [|i IHi] //. rewrite iterate_S [_ ρ]/olty_car/= /eLater IHi//.
   Qed.
 
-  Lemma T_Var Γ x τ:
-    Γ !! x = Some τ →
+  Lemma T_Var Γ x τ
+    (Hx : Γ !! x = Some τ):
     (*──────────────────────*)
     Γ ⊨ of_val (ids x) : τ.|[ren (+x)].
   Proof.
-    iIntros (Hx) "/=". iSplit. eauto using lookup_fv.
-    iIntros "!>" (vs) "#Hg". rewrite hsubst_of_val -wp_value' interp_env_lookup // id_subst. by [].
+    iIntros "/= !>" (ρ) "#Hg". rewrite hsubst_of_val -wp_value' interp_env_lookup // id_subst. by [].
   Qed.
 
   Lemma andstp1 Γ τ1 τ2 i : Γ ⊨ [oAnd τ1 τ2 , i] <: [τ1 , i].
-  Proof. iIntros "!>" (???) "#Hg #[$ _]". Qed.
+  Proof. iIntros "!>" (??) "#Hg #[$ _]". Qed.
 
   Lemma andstp2 Γ τ1 τ2 i : Γ ⊨ [oAnd τ1 τ2 , i] <: [τ2 , i].
-  Proof. iIntros "!>" (???) "#Hg #[_ $]". Qed.
+  Proof. iIntros "!>" (??) "#Hg #[_ $]". Qed.
 End typing.
 
 End OLtyJudgements.
